<?xml version="1.0" encoding="UTF-8"?>

<rdf:RDF
  xmlns="http://www.ideaontology.org/spec/#"
  xmlns:rdf="http://www.w3.org/1999/02/22-rdf-syntax-ns#"
  xmlns:rdfs="http://www.w3.org/2000/01/rdf-schema#"
  xmlns:owl="http://www.w3.org/2002/07/owl#"
  xmlns:foaf="http://xmlns.com/foaf/0.1/"
  xmlns:dcterms="http://purl.org/dc/terms/"
  xmlns:sioc="http://rdfs.org/sioc/ns#"
  xmlns:skos="http://www.w3.org/2008/05/skos#"
  xmlns:rating="http://www.tvblob.com/ratings/#"
  xmlns:tags="http://www.holygoat.co.uk/owl/redwood/0.1/tags/#"
  xmlns:im="http://www.ideaontology.org/spec/#"
>

<!-- 
///////////////////////////////////////////////////////////////////////////////////////
//
// Object Properties
//
///////////////////////////////////////////////////////////////////////////////////////
-->


<owl:ObjectProperty rdf:about="#im:hasAttachment">
	<rdfs:comment>An im:CoreIdea (more specifically: all rdf:Resources) may have documents attached to it (e.g., a screenshot, a process model, technical drawings, etc.) that contains more detailed descriptions of the idea. </rdfs:comment>
	<rdfs:domain rdf:resource="#rdf:Resource"/>
	<rdfs:range rdf:resource="http://xmlns.com/foaf/0.1/document"/>
</owl:ObjectProperty>
<owl:ObjectProperty rdf:about="#im:hasCreator">
	<rdfs:comment>Relates a rdf:Resource to its creator foaf:Person. </rdfs:comment>
	<rdfs:domain rdf:resource="#rdf:Resource"/>
	<rdfs:range rdf:resource="http://xmlns.com/foaf/0.1/person"/>
</owl:ObjectProperty>
<owl:ObjectProperty rdf:about="#im:hasForum">
	<rdfs:comment>An im:CoreIdea may have multiple sioc:forums associated with it where users are discussing the idea. All sioc:items (forum style, blogs, anything) are organized using the SIOC ontology. </rdfs:comment>
	<rdfs:domain rdf:resource="#im:CoreIdea"/>
	<rdfs:range rdf:resource="http://rdfs.org/sioc/ns#Forum"/>
</owl:ObjectProperty>
<owl:ObjectProperty rdf:about="#im:hasOrigin">
	<rdfs:range rdf:resource="#im:Origin"/>
</owl:ObjectProperty>
<owl:ObjectProperty rdf:about="#im:hasRating">
	<rdfs:comment>All innovation related rdf:Resources can be rated. If a rdf:Resource has a r:Rating, this is indicated by im:hasRating. See: tvblob rating. </rdfs:comment>
	<rdfs:domain rdf:resource="#rdf:Resource"/>
	<rdfs:range rdf:resource="http://www.tvblob.com/ratings/#Rating"/>
</owl:ObjectProperty>
<owl:ObjectProperty rdf:about="#im:hasStatus">
	<rdfs:comment>Every im:CoreIdea should have an assigned state which denots the state of this idea. This could mean that an idea is open, evaluated, implemented, etc. </rdfs:comment>
	<rdfs:domain rdf:resource="#im:CoreIdea"/>
	<rdfs:range rdf:resource="#im:Status"/>
</owl:ObjectProperty>
<owl:ObjectProperty rdf:about="#im:hasRealization">
	<rdfs:comment>An im:CoreIdea may be, at a later point in the innovation process, be implemented in a concrete product or service. This is indicated through a im:hasRealization  link to an im:IdeaRealization.</rdfs:comment>
	<rdfs:domain rdf:resource="#im:CoreIdea"/>
	<rdfs:range rdf:resource="#im:IdeaRealization"/>
</owl:ObjectProperty>
<owl:ObjectProperty rdf:about="#im:hasTagging">
	<rdfs:comment>Relates a tag to a rdf:Resource. </rdfs:comment>
	<rdfs:domain rdf:resource="#rdf:Resource"/>
	<rdfs:range rdf:resource="http://www.holygoat.co.uk/owl/redwood/0.1/tags/#Tagging"/>
</owl:ObjectProperty>
<owl:ObjectProperty rdf:about="#im:hasTopic">
	<rdfs:comment>Denots that a given rdf:Resource is related to a skos:Concept. </rdfs:comment>
	<rdfs:domain rdf:resource="#rdf:Resource"/>
	<rdfs:range rdf:resource="http://www.w3.org/2008/05/skos#Concept"/>
</owl:ObjectProperty>
<owl:ObjectProperty rdf:about="#im:isNewVersionOf">
	<rdfs:comment>To account for versioning of ideas and comments different versions of the same idea/comment can be linked to each other indicating that they are &quot;the same&quot; but in different versions. </rdfs:comment>
	<rdfs:domain rdf:resource="#im:CoreIdea"/>
	<rdfs:range rdf:resource="#im:CoreIdea"/>
</owl:ObjectProperty>



<!-- 
///////////////////////////////////////////////////////////////////////////////////////
//
// Data properties
//
///////////////////////////////////////////////////////////////////////////////////////
-->

<owl:DatatypeProperty rdf:about="#im:abstract">
	<rdfs:comment>A medium length abstract describing an im:CoreIdea. For a short title of an idea please use the dc:title attribute and for a longer description of an idea the dc:description attribute of an im:CoreIdea.</rdfs:comment>
	<rdfs:domain rdf:resource="#im:CoreIdea"/>
	<rdfs:range rdf:resource="http://www.w3.org/2000/01/rdf-schema#Literal"/>
</owl:DatatypeProperty>
<owl:DatatypeProperty rdf:about="http://purl.org/dc/terms/date">
	<rdfs:comment>Time this version of an im:CoreIdea has been created.</rdfs:comment>
	<rdfs:domain rdf:resource="#im:CoreIdea"/>
	<rdfs:range rdf:resource="http://www.w3.org/2000/01/rdf-schema#Literal"/>
</owl:DatatypeProperty>
<owl:DatatypeProperty rdf:about="http://purl.org/dc/terms/description">
<rdfs:comment>An account of a rdf:Resource. dc:description is used in the Idea Ontology to assign a textual description to an im:CoreIdea and anim:Status.</rdfs:comment>
	<rdfs:domain rdf:resource="#im:CoreIdea"/>
	<rdfs:domain rdf:resource="#im:Status"/>
	<rdfs:range rdf:resource="http://www.w3.org/2000/01/rdf-schema#Literal"/>
</owl:DatatypeProperty>
<owl:DatatypeProperty rdf:about="http://purl.org/dc/terms/title">
<rdfs:comment>A name given to the resource. dc:title is used in the Idea Ontology to assign a title to im:CoreIdea and im:Status.</rdfs:comment>
	<rdfs:domain rdf:resource="#im:CoreIdea"/>
	<rdfs:domain rdf:resource="#im:Origin"/>
	<rdfs:domain rdf:resource="#im:Status"/>
	<rdfs:range rdf:resource="http://www.w3.org/2000/01/rdf-schema#Literal"/>
</owl:DatatypeProperty>
<owl:DatatypeProperty rdf:about="#im:version">
	<rdfs:comment>Every im:CoreIdea has an im:version number to allow keeping track of different instances of the same idea by means of the im:isNewVersionOf relationship. </rdfs:comment>
	<rdfs:domain rdf:resource="#im:CoreIdea"/>
	<rdfs:range rdf:resource="http://www.w3.org/2000/01/rdf-schema#Literal"/>
</owl:DatatypeProperty>


<!-- 
///////////////////////////////////////////////////////////////////////////////////////
//
// Classes
//
///////////////////////////////////////////////////////////////////////////////////////
-->

<owl:Class rdf:about="#im:CoreIdea">
	<rdfs:subClassOf rdf:resource="#rdf:Resource"/>
	<rdfs:comment>This is the central class of the Idea Ontology. An im:CoreIdea is the entity that holds an idea. To achieve a generic and versatile representation of ideas we chose a hierarchical design with three layers of textual descriptions for a im:CoreIdea: dc:title, im:abstract, and dc:description. All three represent a textual description of the idea but vary in length and detail. Thus, our ontology is able to support very simple tools such as electronic brainstorming where an idea usually consists of no more than one sentence, up to more advanced tools that allow longer descriptions. It is also possible to extend the description with resources such as images, screenshots, or process diagrams: they can be attached as foaf:Documents using the im:hasAttachment relationship. Furthermore, every im:CoreIdea has an associated creation date dc:date and a im:version number to allow keeping track of different instances of the same idea by means of the im:isNewVersionOf relationship. An idea can also have a relationship with sioc:Forum (using im:hasForum) and im:IdeaRealization (using im:hasRalization). Through the sub-classing attributes such im:hasCreator, im:hasRating, and im:hasTagging are inherited from rdf:Resource.</rdfs:comment>
	<rdfs:range rdf:resource="im:abstract"/>
	<rdfs:range rdf:resource="http://purl.org/dc/terms/date"/>
	<rdfs:range rdf:resource="http://purl.org/dc/terms/description"/>
	<rdfs:range rdf:resource="http://purl.org/dc/terms/title"/>
	<rdfs:range rdf:resource="im:isNewVersionOf"/>
	<rdfs:domain rdf:resource="#im:hasForum"/>
	<rdfs:domain rdf:resource="#im:hasRealization"/>
	<rdfs:domain rdf:resource="#im:hasStatus"/>
	<rdfs:domain rdf:resource="#im:isNewVersionOf"/>
</owl:Class>
<owl:Class rdf:about="#im:IdeaRealization">
	<rdfs:comment>To support the full innovation life cycle and to allow for incremental innovations of existing products and services the link between ideas and their resulting realizations must be preserved. Moreover, the back-link from a realization to the original idea allows evaluating various performance measures. For example, it would be possible to identify authors of highly successful ideas. To achieve this tracking across the life cycle our ontology contains an im:IdeaRealization class which is linked to an im:CoreIdea by means of the im:hasRealization object property. The im:IdeaRealization class is a placeholder for whatever is an appropriate means of representing an idea&#39;s realization. In a product environment this may be a product number. In a software-as-a-service environment the idea realization could link to a description of a Web service, for example, using WSDL. The idea described in an im:CoreIdea may be realized as a new product or new service at a later stage of the innovation process. This class is used to link an im:CoreIdea to a realization of that idea.</rdfs:comment>
	<rdfs:range rdf:resource="im:hasRealization"/>
</owl:Class>
<owl:Class rdf:about="#im:Origin">
	<rdfs:label>As one of our Idea Ontology&#39;s main goals is to foster interoperability between various innovation management tools it is necessary to keep track of the application that a given resource originates from. The im:Origin class can be used for this purpose. In this way it can be stated that an idea originates, e.g., from a brainstorming tool, an idea portal on the Web, or another application. The application that the rdf:Resource originates from.</rdfs:label>
	<rdfs:range rdf:resource="im:hasOrigin"/>
	<rdfs:domain rdf:resource="http://purl.org/dc/terms/source"/>
	<rdfs:domain rdf:resource="http://purl.org/dc/terms/title"/>
</owl:Class>
<owl:Class rdf:about="#im:Status">
	<rdfs:comment>In order to track an idea&#39;s progression throughout a submission, evaluation, and implementation process it is necessary to have states associated with an idea. The im:Status class offers this functionality. This class contains a set of instances denoting differnet states an im:CoreIdea can be in. Examples are new, open, evaluated, implemented, etc. </rdfs:comment>
	<rdfs:range rdf:resource="im:hasStatus"/>
	<rdfs:domain rdf:resource="http://purl.org/dc/terms/description"/>
	<rdfs:domain rdf:resource="http://purl.org/dc/terms/title"/>
</owl:Class>
<owl:Class rdf:about="#rdf:Resource">
	<rdfs:comment>Innovation related documents share certain common aspects such as having a topic or being rateable. Thus, all innovation related documents have been subsumed under the class rdf:Resource. Known sub-classes within the context of the Idea Ontology are im:CoreIdea, sioc:Item, and foaf:Document. </rdfs:comment>
	<rdfs:range rdf:resource="im:hasCreator"/>
	<rdfs:range rdf:resource="im:hasTagging"/>
	<rdfs:range rdf:resource="im:hasTopic"/>
	<rdfs:domain rdf:resource="im:hasAttachment"/>
</owl:Class>

</rdf:RDF>



